

I. Структура програми

min	normal
<pre>int main() { return 0; }</pre>	<pre>#include <iostream> #include "windows.h" using namespace std; int main() { SetConsoleCP(1251); SetConsoleOutputCP(1251); // все що потрібно тут!!! // і тут також cout << "ііііі еееее ііііі ііііі"; cout << endl; system("pause"); return 0; }</pre>

№ варіанту	Вигляд функції
01	$f(z) = \cos^2\left(\arctg \frac{1}{z}\right)$
02	$g(x, y) = 5\arctg x - \frac{x^2}{\sqrt[4]{ x+y }}$
03	$f(x, y, z) = y-x \frac{y-\frac{z}{y-x}}{1+(y-x)^2}$
04	$g(x, y) = y^x + \sqrt[3]{ x + y }$
05	$f(x, y) = \lg\left(\sqrt{x} + \frac{x^2}{x^2+y^2} + 2\right)$
06	$g(x, y) = y + \frac{x}{y + \frac{x^2}{y + \frac{x^3}{y}}}$
07	$f(x, y, z) = \lg\left(\sqrt{e^{x-y}} + x^{ y } + z \right)$
08	$g(z) = 1 + \frac{z^2}{3 + \frac{z^2}{5}} + \sin \frac{z}{4}$
09	$f(x, y) = \frac{ \lg x + \cos y }{1 + 2\sin^2 y}$
10	$g(x, y) = \ln\left(y^{\sqrt{x}}\right)\left(x - \frac{y}{y+2}\right)$

11	$f(x, y) = \sqrt{10\left(\sqrt[3]{x} + x^{y-1}\right)}$
12	$g(x, y, z) = \arcsin^2 0.01z + x+y $
13	$f(x, y) = x ^{\frac{y}{x}} - \sqrt[3]{x y }$
14	$g(x, y) = e^{x-1} + \arcsin 0.01y$
15	$f(x, y) = \sqrt{\frac{ y }{e^{-\left(\frac{y}{y+\frac{x}{2}}\right)}}}$
16	$g(x, y, z) = \frac{4y^2 e^{3\sin x}}{3z^2 + \ln x}$
17	$f(x, y, z) = z \frac{\sqrt{y \ln x - 2x^2}}{1 + tg^2 x^2}$
18	$g(x, y, z) = \frac{\ln\left(y + \sqrt{y+x^2}\right)}{z + x^2 + \frac{z+x^2}{e^{\frac{x}{2}}}}$
19	$f(x, z) = \frac{x^2 + 4}{\sin^2 z + \frac{x}{2}}$
20	$g(x, y) = \frac{x + \frac{y}{x^2 + 4}}{y \frac{x-2}{x^2 + 4}}$
21	$f(x, y, z) = \sqrt{2^{x+\sin y} + e^{\lg z}}$

22	$g(x, z) = \sin \left \frac{x+2}{3^{x-2}} \right $
23	$f(x, y) = \frac{1 + \cos^2(x+y)}{ 2y }$
24	$g(x, y) = \frac{\ln x }{\sqrt[3]{ x + y }}$
25	$f(x, y) = x + \frac{y^3}{x + \frac{y^3}{x + y^3}}$
26	$g(x, y) = 2^{-x} \sqrt{x + \sqrt[4]{ y }}$
27	$f(x, z) = \sqrt[3]{\frac{e^{x-1}}{ \sin z }}$
28	$g(x, y, z) = x-y (\sin z + \operatorname{tg} z)$
29	$f(x, y, z) = \sin \frac{x^2}{4} + \frac{e^{-z}}{ x+y }$
30	$g(x, y) = \sqrt[4]{y + \sqrt[3]{x-1}}$
31	$f(x, y, z) = x(\sin \operatorname{arctg} z + \cos^2 y)$
32	$g(x, y, z) = e^{ x-y }(\operatorname{tg}^2 z + 1)^x$